Generalized soundness to arbitrary number of reductions Reduced completeness to `ℱnext` unfolding properties Not using `'a rel` anymore. Always use `'a -> 'a -> bool` instead Still need to find properties for well-foundness

Hygge_Theory.thy
@@ -4,15 +4,8 @@ imports
   "Denotational"
 
 begin
-(** TODO list of desired properties
-  - Soundness
-  - Completeness
-  - Termination
-  - Composition
-  - Decidability
-*)
 
-fun HeronConf_interpretation :: "config \<Rightarrow> run set" ("\<lbrakk> _ \<rbrakk>\<^sub>c\<^sub>o\<^sub>n\<^sub>f") where
+fun HeronConf_interpretation :: "config \<Rightarrow> run set" ("\<lbrakk> _ \<rbrakk>\<^sub>c\<^sub>o\<^sub>n\<^sub>f" 71) where
   "\<lbrakk> \<Gamma>, n \<turnstile> \<Psi> \<triangleright> \<Phi> \<rbrakk>\<^sub>c\<^sub>o\<^sub>n\<^sub>f = \<lbrakk>\<lbrakk> \<Gamma> \<rbrakk>\<rbrakk>\<^sub>s\<^sub>y\<^sub>m\<^sub>r\<^sub>u\<^sub>n \<inter> \<lbrakk>\<lbrakk> \<Psi> \<nabla> n \<rbrakk>\<rbrakk>\<^sub>T\<^sub>E\<^sub>S\<^sub>L \<inter> \<lbrakk>\<lbrakk> \<Phi> \<nabla> Suc n \<rbrakk>\<rbrakk>\<^sub>T\<^sub>E\<^sub>S\<^sub>L"
 
 (* To start solving specification [\<Psi>], we start at configuration [], 0 \<turnstile> \<Psi> \<triangleright> [] *)
@@ -28,10 +21,10 @@ lemma solve_start:
 
 (**) section \<open>Soundness\<close> (**)
 
-theorem reduction_refinement:
+theorem soundness:
   assumes "\<Gamma>\<^sub>1, n\<^sub>1 \<turnstile> \<Psi>\<^sub>1 \<triangleright> \<Phi>\<^sub>1  \<hookrightarrow>  \<Gamma>\<^sub>2, n\<^sub>2 \<turnstile> \<Psi>\<^sub>2 \<triangleright> \<Phi>\<^sub>2"
   shows "\<lbrakk>\<lbrakk> \<Gamma>\<^sub>1 \<rbrakk>\<rbrakk>\<^sub>s\<^sub>y\<^sub>m\<^sub>r\<^sub>u\<^sub>n \<inter> \<lbrakk>\<lbrakk> \<Psi>\<^sub>1 \<nabla> n\<^sub>1 \<rbrakk>\<rbrakk>\<^sub>T\<^sub>E\<^sub>S\<^sub>L \<inter> \<lbrakk>\<lbrakk> \<Phi>\<^sub>1 \<nabla> Suc n\<^sub>1 \<rbrakk>\<rbrakk>\<^sub>T\<^sub>E\<^sub>S\<^sub>L
-         \<supseteq>  \<lbrakk>\<lbrakk> \<Gamma>\<^sub>2 \<rbrakk>\<rbrakk>\<^sub>s\<^sub>y\<^sub>m\<^sub>r\<^sub>u\<^sub>n \<inter> \<lbrakk>\<lbrakk> \<Psi>\<^sub>2 \<nabla> n\<^sub>2 \<rbrakk>\<rbrakk>\<^sub>T\<^sub>E\<^sub>S\<^sub>L \<inter> \<lbrakk>\<lbrakk> \<Phi>\<^sub>2 \<nabla> Suc n\<^sub>2 \<rbrakk>\<rbrakk>\<^sub>T\<^sub>E\<^sub>S\<^sub>L"
+          \<supseteq>  \<lbrakk>\<lbrakk> \<Gamma>\<^sub>2 \<rbrakk>\<rbrakk>\<^sub>s\<^sub>y\<^sub>m\<^sub>r\<^sub>u\<^sub>n \<inter> \<lbrakk>\<lbrakk> \<Psi>\<^sub>2 \<nabla> n\<^sub>2 \<rbrakk>\<rbrakk>\<^sub>T\<^sub>E\<^sub>S\<^sub>L \<inter> \<lbrakk>\<lbrakk> \<Phi>\<^sub>2 \<nabla> Suc n\<^sub>2 \<rbrakk>\<rbrakk>\<^sub>T\<^sub>E\<^sub>S\<^sub>L"
   proof (insert assms, erule operational_semantics_step.cases)
   show "\<And>\<Gamma> n \<Phi>.
        (\<Gamma>\<^sub>1, n\<^sub>1 \<turnstile> \<Psi>\<^sub>1 \<triangleright> \<Phi>\<^sub>1) = (\<Gamma>, n \<turnstile> [] \<triangleright> \<Phi>) \<Longrightarrow>
@@ -175,25 +168,17 @@ theorem reduction_refinement:
     qed
   qed
 
-theorem reduction_refinement':
+theorem soundness':
   assumes "\<S>\<^sub>1 \<hookrightarrow> \<S>\<^sub>2"
   shows "\<lbrakk> \<S>\<^sub>1 \<rbrakk>\<^sub>c\<^sub>o\<^sub>n\<^sub>f \<supseteq> \<lbrakk> \<S>\<^sub>2 \<rbrakk>\<^sub>c\<^sub>o\<^sub>n\<^sub>f"
-  by (metis reduction_refinement HeronConf_interpretation.elims assms)
+  by (metis soundness HeronConf_interpretation.elims assms)
 
-theorem reduction_refinement_rellift:
-  assumes "(\<S>\<^sub>1, \<S>\<^sub>2) \<in> \<hookrightarrow>\<^sup>\<up>"
+theorem soundness_generalized:
+  assumes "\<S>\<^sub>1 \<hookrightarrow>\<^bsup>n\<^esup> \<S>\<^sub>2"
   shows "\<lbrakk> \<S>\<^sub>1 \<rbrakk>\<^sub>c\<^sub>o\<^sub>n\<^sub>f \<supseteq> \<lbrakk> \<S>\<^sub>2 \<rbrakk>\<^sub>c\<^sub>o\<^sub>n\<^sub>f"
-  proof -
-    have "\<S>\<^sub>1 \<hookrightarrow> \<S>\<^sub>2" using assms by auto
-    then show ?thesis using reduction_refinement' by auto
-  qed
-
-theorem reduction_refinement_general:
-  assumes "(\<S>\<^sub>1, \<S>\<^sub>2) \<in> \<hookrightarrow>\<^sup>\<up> ^^ n"
-  shows "\<lbrakk> \<S>\<^sub>1 \<rbrakk>\<^sub>c\<^sub>o\<^sub>n\<^sub>f \<supseteq> \<lbrakk> \<S>\<^sub>2 \<rbrakk>\<^sub>c\<^sub>o\<^sub>n\<^sub>f"
-  proof (insert assms, induct n)
+  proof (insert assms, induct n arbitrary: \<S>\<^sub>2)
     case 0
-    then have *: "(\<S>\<^sub>1, \<S>\<^sub>2) \<in> (\<hookrightarrow>\<^sup>\<up> ^^ 0) \<Longrightarrow> \<S>\<^sub>1 = \<S>\<^sub>2"
+    then have *: "\<S>\<^sub>1 \<hookrightarrow>\<^bsup>0\<^esup> \<S>\<^sub>2 \<Longrightarrow> \<S>\<^sub>1 = \<S>\<^sub>2"
       by auto
     moreover have "\<S>\<^sub>1 = \<S>\<^sub>2" using *
       using "0.prems" by linarith
@@ -203,14 +188,14 @@ theorem reduction_refinement_general:
     then show ?case
       proof -
       fix n :: nat
-      assume hi: "(\<S>\<^sub>1, \<S>\<^sub>2) \<in> \<hookrightarrow>\<^sup>\<up> ^^ n \<Longrightarrow> \<lbrakk> \<S>\<^sub>1 \<rbrakk>\<^sub>c\<^sub>o\<^sub>n\<^sub>f \<supseteq> \<lbrakk> \<S>\<^sub>2 \<rbrakk>\<^sub>c\<^sub>o\<^sub>n\<^sub>f"
-      assume ff: "(\<S>\<^sub>1, \<S>\<^sub>2) \<in> \<hookrightarrow>\<^sup>\<up> ^^ Suc n"
-      obtain \<S>\<^sub>n where f1: "(\<S>\<^sub>1, \<S>\<^sub>n) \<in> \<hookrightarrow>\<^sup>\<up> \<and> (\<S>\<^sub>n, \<S>\<^sub>2) \<in> \<hookrightarrow>\<^sup>\<up>"
-        sorry
+      assume ff: "\<S>\<^sub>1 \<hookrightarrow>\<^bsup>Suc n\<^esup> \<S>\<^sub>2"
+      assume hi: "\<And>\<S>\<^sub>2. \<S>\<^sub>1 \<hookrightarrow>\<^bsup>n\<^esup> \<S>\<^sub>2 \<Longrightarrow> \<lbrakk> \<S>\<^sub>2 \<rbrakk>\<^sub>c\<^sub>o\<^sub>n\<^sub>f \<subseteq> \<lbrakk> \<S>\<^sub>1 \<rbrakk>\<^sub>c\<^sub>o\<^sub>n\<^sub>f"
+      obtain \<S>\<^sub>n where red_decomp: "\<S>\<^sub>1 \<hookrightarrow>\<^bsup>n\<^esup> \<S>\<^sub>n \<and> \<S>\<^sub>n \<hookrightarrow> \<S>\<^sub>2"
+        using ff by auto
       then have "\<lbrakk> \<S>\<^sub>1 \<rbrakk>\<^sub>c\<^sub>o\<^sub>n\<^sub>f \<supseteq> \<lbrakk> \<S>\<^sub>n \<rbrakk>\<^sub>c\<^sub>o\<^sub>n\<^sub>f"
-        using hi by (simp add: reduction_refinement_rellift)
+        using hi by (metis (no_types, lifting) ff relpowp_Suc_E someI_ex)
       also have "\<lbrakk> \<S>\<^sub>n \<rbrakk>\<^sub>c\<^sub>o\<^sub>n\<^sub>f \<supseteq> \<lbrakk> \<S>\<^sub>2 \<rbrakk>\<^sub>c\<^sub>o\<^sub>n\<^sub>f"
-        using hi f1 reduction_refinement_rellift by auto
+        by (simp add: red_decomp soundness')
       ultimately show "\<lbrakk> \<S>\<^sub>1 \<rbrakk>\<^sub>c\<^sub>o\<^sub>n\<^sub>f \<supseteq> \<lbrakk> \<S>\<^sub>2 \<rbrakk>\<^sub>c\<^sub>o\<^sub>n\<^sub>f"
         by auto
       qed
@@ -218,23 +203,187 @@ theorem reduction_refinement_general:
 
 (**) section \<open>Completeness\<close> (**)
 
-abbreviation next_solve :: "config \<Rightarrow> config set" ("\<F>\<^sub>n\<^sub>e\<^sub>x\<^sub>t _") where
+abbreviation Fnext_solve :: "config \<Rightarrow> config set" ("\<F>\<^sub>n\<^sub>e\<^sub>x\<^sub>t _") where
   "\<F>\<^sub>n\<^sub>e\<^sub>x\<^sub>t \<S> \<equiv> { \<S>'. \<S> \<hookrightarrow> \<S>' }"
+
+lemma Fnext_solve_instant:
+  shows "\<F>\<^sub>n\<^sub>e\<^sub>x\<^sub>t (\<Gamma>, n \<turnstile> [] \<triangleright> \<Phi>)
+          = { \<Gamma>, Suc n \<turnstile> \<Phi> \<triangleright> [] }"
+  sorry
+
+lemma Fnext_solve_sporadic:
+  shows "\<F>\<^sub>n\<^sub>e\<^sub>x\<^sub>t (\<Gamma>, n \<turnstile> (K sporadic \<tau>) # \<Psi> \<triangleright> \<Phi>)
+          = { \<Gamma>, n \<turnstile> \<Psi> \<triangleright> (K sporadic \<tau>) # \<Phi>,
+              K \<Up> n # K \<Down> n @ \<lfloor>\<tau>\<rfloor> # \<Gamma>, n \<turnstile> \<Psi> \<triangleright> \<Phi> }"
+  sorry
+
+lemma Fnext_solve_sporadicon:
+  shows "\<F>\<^sub>n\<^sub>e\<^sub>x\<^sub>t (\<Gamma>, n \<turnstile> (K\<^sub>1 sporadic \<tau> on K\<^sub>2) # \<Psi> \<triangleright> \<Phi>)
+          = { \<Gamma>, n \<turnstile> \<Psi> \<triangleright> (K\<^sub>1 sporadic \<tau> on K\<^sub>2) # \<Phi>,
+              K\<^sub>1 \<Up> n # K\<^sub>2 \<Down> n @ \<tau> # \<Gamma>, n \<turnstile> \<Psi> \<triangleright> \<Phi> }"
+  sorry
+
+lemma Fnext_solve_tagrel:
+  shows "\<F>\<^sub>n\<^sub>e\<^sub>x\<^sub>t (\<Gamma>, n \<turnstile> (tag-relation K\<^sub>1 = \<alpha> * K\<^sub>2 + \<beta>) # \<Psi> \<triangleright> \<Phi>)
+          = { (\<tau>\<^sub>v\<^sub>a\<^sub>r(K\<^sub>1, n) \<doteq> \<alpha> * \<tau>\<^sub>v\<^sub>a\<^sub>r(K\<^sub>2, n) + \<beta>) # \<Gamma>, n \<turnstile> \<Psi> \<triangleright> (tag-relation K\<^sub>1 = \<alpha> * K\<^sub>2 + \<beta>) # \<Phi> }"
+  sorry
+
+lemma Fnext_solve_implies:
+  shows "\<F>\<^sub>n\<^sub>e\<^sub>x\<^sub>t (\<Gamma>, n \<turnstile> (K\<^sub>1 implies K\<^sub>2) # \<Psi> \<triangleright> \<Phi>)
+          = { K\<^sub>1 \<not>\<Up> n # \<Gamma>, n \<turnstile> \<Psi> \<triangleright> (K\<^sub>1 implies K\<^sub>2) # \<Phi>,
+              K\<^sub>1 \<Up> n # K\<^sub>2 \<Up> n # \<Gamma>, n \<turnstile> \<Psi> \<triangleright> (K\<^sub>1 implies K\<^sub>2) # \<Phi>}"
+  sorry
+
+lemma Fnext_solve_timedelayed:
+  shows "\<F>\<^sub>n\<^sub>e\<^sub>x\<^sub>t (\<Gamma>, n \<turnstile> (K\<^sub>1 time-delayed by \<delta>\<tau> on K\<^sub>2 implies K\<^sub>3) # \<Psi> \<triangleright> \<Phi>)
+          = { K\<^sub>1 \<not>\<Up> n # \<Gamma>, n \<turnstile> \<Psi> \<triangleright> (K\<^sub>1 time-delayed by \<delta>\<tau> on K\<^sub>2 implies K\<^sub>3) # \<Phi>,
+              K\<^sub>1 \<Up> n # \<Gamma>, n \<turnstile> (K\<^sub>3 sporadic \<lfloor>\<tau>\<^sub>v\<^sub>a\<^sub>r(K\<^sub>2, n) \<oplus> \<delta>\<tau>\<rfloor> on K\<^sub>2) # \<Psi> \<triangleright> (K\<^sub>1 time-delayed by \<delta>\<tau> on K\<^sub>2 implies K\<^sub>3) # \<Phi> }"
+  sorry
+
+lemma HeronConf_interp_at_index_sporadic_cases:
+  shows "\<lbrakk> \<Gamma>, n \<turnstile> (K sporadic \<tau>) # \<Psi> \<triangleright> \<Phi> \<rbrakk>\<^sub>c\<^sub>o\<^sub>n\<^sub>f
+          = \<lbrakk> \<Gamma>, n \<turnstile> \<Psi> \<triangleright> (K sporadic \<tau>) # \<Phi> \<rbrakk>\<^sub>c\<^sub>o\<^sub>n\<^sub>f
+          \<union> \<lbrakk> K \<Up> n # K \<Down> n @ \<lfloor>\<tau>\<rfloor> # \<Gamma>, n \<turnstile> \<Psi> \<triangleright> \<Phi> \<rbrakk>\<^sub>c\<^sub>o\<^sub>n\<^sub>f"
+  proof -
+    have "\<lbrakk> \<Gamma>, n \<turnstile> (K sporadic \<tau>) # \<Psi> \<triangleright> \<Phi> \<rbrakk>\<^sub>c\<^sub>o\<^sub>n\<^sub>f = \<lbrakk>\<lbrakk> \<Gamma> \<rbrakk>\<rbrakk>\<^sub>s\<^sub>y\<^sub>m\<^sub>r\<^sub>u\<^sub>n \<inter> \<lbrakk>\<lbrakk> (K sporadic \<tau>) # \<Psi> \<nabla> n \<rbrakk>\<rbrakk>\<^sub>T\<^sub>E\<^sub>S\<^sub>L \<inter> \<lbrakk>\<lbrakk> \<Phi> \<nabla> Suc n \<rbrakk>\<rbrakk>\<^sub>T\<^sub>E\<^sub>S\<^sub>L"
+      by simp
+    moreover have "\<lbrakk> \<Gamma>, n \<turnstile> \<Psi> \<triangleright> (K sporadic \<tau>) # \<Phi> \<rbrakk>\<^sub>c\<^sub>o\<^sub>n\<^sub>f = \<lbrakk>\<lbrakk> \<Gamma> \<rbrakk>\<rbrakk>\<^sub>s\<^sub>y\<^sub>m\<^sub>r\<^sub>u\<^sub>n \<inter> \<lbrakk>\<lbrakk> \<Psi> \<nabla> n \<rbrakk>\<rbrakk>\<^sub>T\<^sub>E\<^sub>S\<^sub>L \<inter> \<lbrakk>\<lbrakk> (K sporadic \<tau>) # \<Phi> \<nabla> Suc n \<rbrakk>\<rbrakk>\<^sub>T\<^sub>E\<^sub>S\<^sub>L"
+      by simp
+    moreover have "\<lbrakk> K \<Up> n # K \<Down> n @ \<lfloor>\<tau>\<rfloor> # \<Gamma>, n \<turnstile> \<Psi> \<triangleright> \<Phi> \<rbrakk>\<^sub>c\<^sub>o\<^sub>n\<^sub>f = \<lbrakk>\<lbrakk> K \<Up> n # K \<Down> n @ \<lfloor>\<tau>\<rfloor> # \<Gamma> \<rbrakk>\<rbrakk>\<^sub>s\<^sub>y\<^sub>m\<^sub>r\<^sub>u\<^sub>n \<inter> \<lbrakk>\<lbrakk> \<Psi> \<nabla> n \<rbrakk>\<rbrakk>\<^sub>T\<^sub>E\<^sub>S\<^sub>L \<inter> \<lbrakk>\<lbrakk> \<Phi> \<nabla> Suc n \<rbrakk>\<rbrakk>\<^sub>T\<^sub>E\<^sub>S\<^sub>L"
+      by simp
+    ultimately show ?thesis
+    proof -
+      have "(\<lbrakk> K \<Up> n \<rbrakk>\<^sub>s\<^sub>y\<^sub>m\<^sub>r\<^sub>u\<^sub>n \<inter> \<lbrakk> K \<Down> n @ \<lfloor> \<tau> \<rfloor> \<rbrakk>\<^sub>s\<^sub>y\<^sub>m\<^sub>r\<^sub>u\<^sub>n \<union> \<lbrakk> K sporadic \<tau> \<nabla> Suc n \<rbrakk>\<^sub>T\<^sub>E\<^sub>S\<^sub>L) \<inter> \<lbrakk>\<lbrakk> \<Psi> \<nabla> n \<rbrakk>\<rbrakk>\<^sub>T\<^sub>E\<^sub>S\<^sub>L = \<lbrakk>\<lbrakk> (K sporadic \<tau>) # \<Psi> \<nabla> n \<rbrakk>\<rbrakk>\<^sub>T\<^sub>E\<^sub>S\<^sub>L"
+        using TESL_interp_at_index_sporadic_cases TESL_interpretation_at_index_cons_morph by blast
+  then have "\<lbrakk> \<Gamma>, n \<turnstile> (K sporadic \<tau>) # \<Psi> \<triangleright> \<Phi> \<rbrakk>\<^sub>c\<^sub>o\<^sub>n\<^sub>f = (\<lbrakk>\<lbrakk> K \<Up> n # K \<Down> n @ \<lfloor> \<tau> \<rfloor> # \<Gamma> \<rbrakk>\<rbrakk>\<^sub>s\<^sub>y\<^sub>m\<^sub>r\<^sub>u\<^sub>n \<inter> \<lbrakk>\<lbrakk> \<Psi> \<nabla> n \<rbrakk>\<rbrakk>\<^sub>T\<^sub>E\<^sub>S\<^sub>L \<union> \<lbrakk>\<lbrakk> \<Gamma> \<rbrakk>\<rbrakk>\<^sub>s\<^sub>y\<^sub>m\<^sub>r\<^sub>u\<^sub>n \<inter> \<lbrakk>\<lbrakk> \<Psi> \<nabla> n \<rbrakk>\<rbrakk>\<^sub>T\<^sub>E\<^sub>S\<^sub>L \<inter> \<lbrakk> K sporadic \<tau> \<nabla> Suc n \<rbrakk>\<^sub>T\<^sub>E\<^sub>S\<^sub>L) \<inter> \<lbrakk>\<lbrakk> \<Phi> \<nabla> Suc n \<rbrakk>\<rbrakk>\<^sub>T\<^sub>E\<^sub>S\<^sub>L"
+    by auto
+      then show ?thesis
+        by (simp add: Int_Un_distrib2 Int_assoc Un_commute)
+    qed
+  qed
+
+lemma HeronConf_interp_at_index_sporadicon_cases:
+  shows "\<lbrakk> \<Gamma>, n \<turnstile> (K\<^sub>1 sporadic \<tau> on K\<^sub>2) # \<Psi> \<triangleright> \<Phi> \<rbrakk>\<^sub>c\<^sub>o\<^sub>n\<^sub>f
+          = \<lbrakk> \<Gamma>, n \<turnstile> \<Psi> \<triangleright> (K\<^sub>1 sporadic \<tau> on K\<^sub>2) # \<Phi> \<rbrakk>\<^sub>c\<^sub>o\<^sub>n\<^sub>f
+          \<union> \<lbrakk> K\<^sub>1 \<Up> n # K\<^sub>2 \<Down> n @ \<tau> # \<Gamma>, n \<turnstile> \<Psi> \<triangleright> \<Phi> \<rbrakk>\<^sub>c\<^sub>o\<^sub>n\<^sub>f"
+  proof -
+    have "\<lbrakk> \<Gamma>, n \<turnstile> (K\<^sub>1 sporadic \<tau> on K\<^sub>2) # \<Psi> \<triangleright> \<Phi> \<rbrakk>\<^sub>c\<^sub>o\<^sub>n\<^sub>f = \<lbrakk>\<lbrakk> \<Gamma> \<rbrakk>\<rbrakk>\<^sub>s\<^sub>y\<^sub>m\<^sub>r\<^sub>u\<^sub>n \<inter> \<lbrakk>\<lbrakk> (K\<^sub>1 sporadic \<tau> on K\<^sub>2) # \<Psi> \<nabla> n \<rbrakk>\<rbrakk>\<^sub>T\<^sub>E\<^sub>S\<^sub>L \<inter> \<lbrakk>\<lbrakk> \<Phi> \<nabla> Suc n \<rbrakk>\<rbrakk>\<^sub>T\<^sub>E\<^sub>S\<^sub>L"
+      by simp
+    moreover have "\<lbrakk> \<Gamma>, n \<turnstile> \<Psi> \<triangleright> (K\<^sub>1 sporadic \<tau> on K\<^sub>2) # \<Phi> \<rbrakk>\<^sub>c\<^sub>o\<^sub>n\<^sub>f = \<lbrakk>\<lbrakk> \<Gamma> \<rbrakk>\<rbrakk>\<^sub>s\<^sub>y\<^sub>m\<^sub>r\<^sub>u\<^sub>n \<inter> \<lbrakk>\<lbrakk> \<Psi> \<nabla> n \<rbrakk>\<rbrakk>\<^sub>T\<^sub>E\<^sub>S\<^sub>L \<inter> \<lbrakk>\<lbrakk> (K\<^sub>1 sporadic \<tau> on K\<^sub>2) # \<Phi> \<nabla> Suc n \<rbrakk>\<rbrakk>\<^sub>T\<^sub>E\<^sub>S\<^sub>L"
+      by simp
+    moreover have "\<lbrakk> K\<^sub>1 \<Up> n # K\<^sub>2 \<Down> n @ \<tau> # \<Gamma>, n \<turnstile> \<Psi> \<triangleright> \<Phi> \<rbrakk>\<^sub>c\<^sub>o\<^sub>n\<^sub>f = \<lbrakk>\<lbrakk> K\<^sub>1 \<Up> n # K\<^sub>2 \<Down> n @ \<tau> # \<Gamma> \<rbrakk>\<rbrakk>\<^sub>s\<^sub>y\<^sub>m\<^sub>r\<^sub>u\<^sub>n \<inter> \<lbrakk>\<lbrakk> \<Psi> \<nabla> n \<rbrakk>\<rbrakk>\<^sub>T\<^sub>E\<^sub>S\<^sub>L \<inter> \<lbrakk>\<lbrakk> \<Phi> \<nabla> Suc n \<rbrakk>\<rbrakk>\<^sub>T\<^sub>E\<^sub>S\<^sub>L"
+      by simp
+    ultimately show ?thesis
+    proof -
+      have "(\<lbrakk> K\<^sub>1 \<Up> n \<rbrakk>\<^sub>s\<^sub>y\<^sub>m\<^sub>r\<^sub>u\<^sub>n \<inter> \<lbrakk> K\<^sub>2 \<Down> n @ \<tau> \<rbrakk>\<^sub>s\<^sub>y\<^sub>m\<^sub>r\<^sub>u\<^sub>n \<union> \<lbrakk> K\<^sub>1 sporadic \<tau> on K\<^sub>2 \<nabla> Suc n \<rbrakk>\<^sub>T\<^sub>E\<^sub>S\<^sub>L) \<inter> (\<lbrakk>\<lbrakk> \<Gamma> \<rbrakk>\<rbrakk>\<^sub>s\<^sub>y\<^sub>m\<^sub>r\<^sub>u\<^sub>n \<inter> \<lbrakk>\<lbrakk> \<Psi> \<nabla> n \<rbrakk>\<rbrakk>\<^sub>T\<^sub>E\<^sub>S\<^sub>L) = \<lbrakk> K\<^sub>1 sporadic \<tau> on K\<^sub>2 \<nabla> n \<rbrakk>\<^sub>T\<^sub>E\<^sub>S\<^sub>L \<inter> (\<lbrakk>\<lbrakk> \<Psi> \<nabla> n \<rbrakk>\<rbrakk>\<^sub>T\<^sub>E\<^sub>S\<^sub>L \<inter> \<lbrakk>\<lbrakk> \<Gamma> \<rbrakk>\<rbrakk>\<^sub>s\<^sub>y\<^sub>m\<^sub>r\<^sub>u\<^sub>n)"
+        using TESL_interp_at_index_sporadicon_cases by blast
+      then have "\<lbrakk>\<lbrakk> K\<^sub>1 \<Up> n # K\<^sub>2 \<Down> n @ \<tau> # \<Gamma> \<rbrakk>\<rbrakk>\<^sub>s\<^sub>y\<^sub>m\<^sub>r\<^sub>u\<^sub>n \<inter> \<lbrakk>\<lbrakk> \<Psi> \<nabla> n \<rbrakk>\<rbrakk>\<^sub>T\<^sub>E\<^sub>S\<^sub>L \<union> \<lbrakk>\<lbrakk> \<Gamma> \<rbrakk>\<rbrakk>\<^sub>s\<^sub>y\<^sub>m\<^sub>r\<^sub>u\<^sub>n \<inter> \<lbrakk>\<lbrakk> \<Psi> \<nabla> n \<rbrakk>\<rbrakk>\<^sub>T\<^sub>E\<^sub>S\<^sub>L \<inter> \<lbrakk> K\<^sub>1 sporadic \<tau> on K\<^sub>2 \<nabla> Suc n \<rbrakk>\<^sub>T\<^sub>E\<^sub>S\<^sub>L = \<lbrakk>\<lbrakk> (K\<^sub>1 sporadic \<tau> on K\<^sub>2) # \<Psi> \<nabla> n \<rbrakk>\<rbrakk>\<^sub>T\<^sub>E\<^sub>S\<^sub>L \<inter> \<lbrakk>\<lbrakk> \<Gamma> \<rbrakk>\<rbrakk>\<^sub>s\<^sub>y\<^sub>m\<^sub>r\<^sub>u\<^sub>n"
+        by auto
+      then show ?thesis
+        by auto
+    qed
+  qed
+
+lemma HeronConf_interp_at_index_tagrel_cases:
+  shows "\<lbrakk> \<Gamma>, n \<turnstile> (tag-relation K\<^sub>1 = \<alpha> * K\<^sub>2 + \<beta>) # \<Psi> \<triangleright> \<Phi> \<rbrakk>\<^sub>c\<^sub>o\<^sub>n\<^sub>f
+          = \<lbrakk> (\<tau>\<^sub>v\<^sub>a\<^sub>r(K\<^sub>1, n) \<doteq> \<alpha> * \<tau>\<^sub>v\<^sub>a\<^sub>r(K\<^sub>2, n) + \<beta>) # \<Gamma>, n \<turnstile> \<Psi> \<triangleright> (tag-relation K\<^sub>1 = \<alpha> * K\<^sub>2 + \<beta>) # \<Phi> \<rbrakk>\<^sub>c\<^sub>o\<^sub>n\<^sub>f"
+  proof -
+    have "\<lbrakk> \<Gamma>, n \<turnstile> (tag-relation K\<^sub>1 = \<alpha> * K\<^sub>2 + \<beta>) # \<Psi> \<triangleright> \<Phi> \<rbrakk>\<^sub>c\<^sub>o\<^sub>n\<^sub>f = \<lbrakk>\<lbrakk> \<Gamma> \<rbrakk>\<rbrakk>\<^sub>s\<^sub>y\<^sub>m\<^sub>r\<^sub>u\<^sub>n \<inter> \<lbrakk>\<lbrakk> (tag-relation K\<^sub>1 = \<alpha> * K\<^sub>2 + \<beta>) # \<Psi> \<nabla> n \<rbrakk>\<rbrakk>\<^sub>T\<^sub>E\<^sub>S\<^sub>L \<inter> \<lbrakk>\<lbrakk> \<Phi> \<nabla> Suc n \<rbrakk>\<rbrakk>\<^sub>T\<^sub>E\<^sub>S\<^sub>L"
+      by simp
+    moreover have "\<lbrakk> (\<tau>\<^sub>v\<^sub>a\<^sub>r(K\<^sub>1, n) \<doteq> \<alpha> * \<tau>\<^sub>v\<^sub>a\<^sub>r(K\<^sub>2, n) + \<beta>) # \<Gamma>, n \<turnstile> \<Psi> \<triangleright> (tag-relation K\<^sub>1 = \<alpha> * K\<^sub>2 + \<beta>) # \<Phi> \<rbrakk>\<^sub>c\<^sub>o\<^sub>n\<^sub>f
+                      = \<lbrakk>\<lbrakk> (\<tau>\<^sub>v\<^sub>a\<^sub>r(K\<^sub>1, n) \<doteq> \<alpha> * \<tau>\<^sub>v\<^sub>a\<^sub>r(K\<^sub>2, n) + \<beta>) # \<Gamma> \<rbrakk>\<rbrakk>\<^sub>s\<^sub>y\<^sub>m\<^sub>r\<^sub>u\<^sub>n \<inter> \<lbrakk>\<lbrakk> \<Psi> \<nabla> n \<rbrakk>\<rbrakk>\<^sub>T\<^sub>E\<^sub>S\<^sub>L \<inter> \<lbrakk>\<lbrakk> (tag-relation K\<^sub>1 = \<alpha> * K\<^sub>2 + \<beta>) # \<Phi> \<nabla> Suc n \<rbrakk>\<rbrakk>\<^sub>T\<^sub>E\<^sub>S\<^sub>L"
+      by simp
+    ultimately show ?thesis
+    proof -
+      have "\<lbrakk> \<tau>\<^sub>v\<^sub>a\<^sub>r (K\<^sub>1, n) \<doteq> \<alpha> * \<tau>\<^sub>v\<^sub>a\<^sub>r (K\<^sub>2, n) + \<beta> \<rbrakk>\<^sub>s\<^sub>y\<^sub>m\<^sub>r\<^sub>u\<^sub>n \<inter> \<lbrakk> tag-relation K\<^sub>1 = \<alpha> * K\<^sub>2 + \<beta> \<nabla> Suc n \<rbrakk>\<^sub>T\<^sub>E\<^sub>S\<^sub>L \<inter> \<lbrakk>\<lbrakk> \<Psi> \<nabla> n \<rbrakk>\<rbrakk>\<^sub>T\<^sub>E\<^sub>S\<^sub>L = \<lbrakk>\<lbrakk> (tag-relation K\<^sub>1 = \<alpha> * K\<^sub>2 + \<beta>) # \<Psi> \<nabla> n \<rbrakk>\<rbrakk>\<^sub>T\<^sub>E\<^sub>S\<^sub>L"
+        using TESL_interp_at_index_tagrel_cases TESL_interpretation_at_index_cons_morph by blast
+      then show ?thesis
+        by auto
+    qed
+  qed
+
+lemma HeronConf_interp_at_index_implies_cases:
+  shows "\<lbrakk> \<Gamma>, n \<turnstile> (K\<^sub>1 implies K\<^sub>2) # \<Psi> \<triangleright> \<Phi> \<rbrakk>\<^sub>c\<^sub>o\<^sub>n\<^sub>f
+          = \<lbrakk> K\<^sub>1 \<not>\<Up> n # \<Gamma>, n \<turnstile> \<Psi> \<triangleright> (K\<^sub>1 implies K\<^sub>2) # \<Phi> \<rbrakk>\<^sub>c\<^sub>o\<^sub>n\<^sub>f
+          \<union> \<lbrakk> K\<^sub>1 \<Up> n # K\<^sub>2 \<Up> n # \<Gamma>, n \<turnstile> \<Psi> \<triangleright> (K\<^sub>1 implies K\<^sub>2) # \<Phi> \<rbrakk>\<^sub>c\<^sub>o\<^sub>n\<^sub>f"
+  proof -
+    have "\<lbrakk> \<Gamma>, n \<turnstile> (K\<^sub>1 implies K\<^sub>2) # \<Psi> \<triangleright> \<Phi> \<rbrakk>\<^sub>c\<^sub>o\<^sub>n\<^sub>f = \<lbrakk>\<lbrakk> \<Gamma> \<rbrakk>\<rbrakk>\<^sub>s\<^sub>y\<^sub>m\<^sub>r\<^sub>u\<^sub>n \<inter> \<lbrakk>\<lbrakk> (K\<^sub>1 implies K\<^sub>2) # \<Psi> \<nabla> n \<rbrakk>\<rbrakk>\<^sub>T\<^sub>E\<^sub>S\<^sub>L \<inter> \<lbrakk>\<lbrakk> \<Phi> \<nabla> Suc n \<rbrakk>\<rbrakk>\<^sub>T\<^sub>E\<^sub>S\<^sub>L"
+      by simp
+    moreover have "\<lbrakk> K\<^sub>1 \<not>\<Up> n # \<Gamma>, n \<turnstile> \<Psi> \<triangleright> (K\<^sub>1 implies K\<^sub>2) # \<Phi> \<rbrakk>\<^sub>c\<^sub>o\<^sub>n\<^sub>f = \<lbrakk>\<lbrakk> K\<^sub>1 \<not>\<Up> n # \<Gamma> \<rbrakk>\<rbrakk>\<^sub>s\<^sub>y\<^sub>m\<^sub>r\<^sub>u\<^sub>n \<inter> \<lbrakk>\<lbrakk> \<Psi> \<nabla> n \<rbrakk>\<rbrakk>\<^sub>T\<^sub>E\<^sub>S\<^sub>L \<inter> \<lbrakk>\<lbrakk> (K\<^sub>1 implies K\<^sub>2) # \<Phi> \<nabla> Suc n \<rbrakk>\<rbrakk>\<^sub>T\<^sub>E\<^sub>S\<^sub>L"
+      by simp
+    moreover have "\<lbrakk> K\<^sub>1 \<Up> n # K\<^sub>2 \<Up> n # \<Gamma>, n \<turnstile> \<Psi> \<triangleright> (K\<^sub>1 implies K\<^sub>2) # \<Phi> \<rbrakk>\<^sub>c\<^sub>o\<^sub>n\<^sub>f = \<lbrakk>\<lbrakk> K\<^sub>1 \<Up> n # K\<^sub>2 \<Up> n # \<Gamma> \<rbrakk>\<rbrakk>\<^sub>s\<^sub>y\<^sub>m\<^sub>r\<^sub>u\<^sub>n \<inter> \<lbrakk>\<lbrakk> \<Psi> \<nabla> n \<rbrakk>\<rbrakk>\<^sub>T\<^sub>E\<^sub>S\<^sub>L \<inter> \<lbrakk>\<lbrakk> (K\<^sub>1 implies K\<^sub>2) # \<Phi> \<nabla> Suc n \<rbrakk>\<rbrakk>\<^sub>T\<^sub>E\<^sub>S\<^sub>L"
+      by simp
+    ultimately show ?thesis
+    proof -
+      have f1: "(\<lbrakk> K\<^sub>1 \<not>\<Up> n \<rbrakk>\<^sub>s\<^sub>y\<^sub>m\<^sub>r\<^sub>u\<^sub>n \<union> \<lbrakk> K\<^sub>1 \<Up> n \<rbrakk>\<^sub>s\<^sub>y\<^sub>m\<^sub>r\<^sub>u\<^sub>n \<inter> \<lbrakk> K\<^sub>2 \<Up> n \<rbrakk>\<^sub>s\<^sub>y\<^sub>m\<^sub>r\<^sub>u\<^sub>n) \<inter> \<lbrakk> K\<^sub>1 implies K\<^sub>2 \<nabla> Suc n \<rbrakk>\<^sub>T\<^sub>E\<^sub>S\<^sub>L \<inter> (\<lbrakk>\<lbrakk> \<Psi> \<nabla> n \<rbrakk>\<rbrakk>\<^sub>T\<^sub>E\<^sub>S\<^sub>L \<inter> \<lbrakk>\<lbrakk> \<Phi> \<nabla> Suc n \<rbrakk>\<rbrakk>\<^sub>T\<^sub>E\<^sub>S\<^sub>L) = \<lbrakk>\<lbrakk> (K\<^sub>1 implies K\<^sub>2) # \<Psi> \<nabla> n \<rbrakk>\<rbrakk>\<^sub>T\<^sub>E\<^sub>S\<^sub>L \<inter> \<lbrakk>\<lbrakk> \<Phi> \<nabla> Suc n \<rbrakk>\<rbrakk>\<^sub>T\<^sub>E\<^sub>S\<^sub>L"
+        using TESL_interp_at_index_implies_cases TESL_interpretation_at_index_cons_morph by blast
+      have "\<lbrakk> K\<^sub>1 \<not>\<Up> n \<rbrakk>\<^sub>s\<^sub>y\<^sub>m\<^sub>r\<^sub>u\<^sub>n \<inter> \<lbrakk>\<lbrakk> \<Gamma> \<rbrakk>\<rbrakk>\<^sub>s\<^sub>y\<^sub>m\<^sub>r\<^sub>u\<^sub>n \<union> \<lbrakk> K\<^sub>1 \<Up> n \<rbrakk>\<^sub>s\<^sub>y\<^sub>m\<^sub>r\<^sub>u\<^sub>n \<inter> \<lbrakk>\<lbrakk> K\<^sub>2 \<Up> n # \<Gamma> \<rbrakk>\<rbrakk>\<^sub>s\<^sub>y\<^sub>m\<^sub>r\<^sub>u\<^sub>n = (\<lbrakk> K\<^sub>1 \<not>\<Up> n \<rbrakk>\<^sub>s\<^sub>y\<^sub>m\<^sub>r\<^sub>u\<^sub>n \<union> \<lbrakk> K\<^sub>1 \<Up> n \<rbrakk>\<^sub>s\<^sub>y\<^sub>m\<^sub>r\<^sub>u\<^sub>n \<inter> \<lbrakk> K\<^sub>2 \<Up> n \<rbrakk>\<^sub>s\<^sub>y\<^sub>m\<^sub>r\<^sub>u\<^sub>n) \<inter> \<lbrakk>\<lbrakk> \<Gamma> \<rbrakk>\<rbrakk>\<^sub>s\<^sub>y\<^sub>m\<^sub>r\<^sub>u\<^sub>n"
+        by force
+      then have "\<lbrakk> \<Gamma>, n \<turnstile> (K\<^sub>1 implies K\<^sub>2) # \<Psi> \<triangleright> \<Phi> \<rbrakk>\<^sub>c\<^sub>o\<^sub>n\<^sub>f = (\<lbrakk> K\<^sub>1 \<not>\<Up> n \<rbrakk>\<^sub>s\<^sub>y\<^sub>m\<^sub>r\<^sub>u\<^sub>n \<inter> \<lbrakk>\<lbrakk> \<Gamma> \<rbrakk>\<rbrakk>\<^sub>s\<^sub>y\<^sub>m\<^sub>r\<^sub>u\<^sub>n \<union> \<lbrakk> K\<^sub>1 \<Up> n \<rbrakk>\<^sub>s\<^sub>y\<^sub>m\<^sub>r\<^sub>u\<^sub>n \<inter> \<lbrakk>\<lbrakk> K\<^sub>2 \<Up> n # \<Gamma> \<rbrakk>\<rbrakk>\<^sub>s\<^sub>y\<^sub>m\<^sub>r\<^sub>u\<^sub>n) \<inter> (\<lbrakk>\<lbrakk> \<Psi> \<nabla> n \<rbrakk>\<rbrakk>\<^sub>T\<^sub>E\<^sub>S\<^sub>L \<inter> \<lbrakk>\<lbrakk> (K\<^sub>1 implies K\<^sub>2) # \<Phi> \<nabla> Suc n \<rbrakk>\<rbrakk>\<^sub>T\<^sub>E\<^sub>S\<^sub>L)"
+        using f1 by (simp add: inf_left_commute inf_sup_aci(2))
+      then show ?thesis
+        by (simp add: Int_Un_distrib2 inf_sup_aci(2))
+    qed
+  qed
+
+lemma HeronConf_interp_at_index_timedelayed_cases:
+  shows "\<lbrakk> \<Gamma>, n \<turnstile> (K\<^sub>1 time-delayed by \<delta>\<tau> on K\<^sub>2 implies K\<^sub>3) # \<Psi> \<triangleright> \<Phi> \<rbrakk>\<^sub>c\<^sub>o\<^sub>n\<^sub>f
+          = \<lbrakk> K\<^sub>1 \<not>\<Up> n # \<Gamma>, n \<turnstile> \<Psi> \<triangleright> (K\<^sub>1 time-delayed by \<delta>\<tau> on K\<^sub>2 implies K\<^sub>3) # \<Phi> \<rbrakk>\<^sub>c\<^sub>o\<^sub>n\<^sub>f
+          \<union> \<lbrakk> K\<^sub>1 \<Up> n # \<Gamma>, n \<turnstile> (K\<^sub>3 sporadic \<lfloor>\<tau>\<^sub>v\<^sub>a\<^sub>r(K\<^sub>2, n) \<oplus> \<delta>\<tau>\<rfloor> on K\<^sub>2) # \<Psi> \<triangleright> (K\<^sub>1 time-delayed by \<delta>\<tau> on K\<^sub>2 implies K\<^sub>3) # \<Phi> \<rbrakk>\<^sub>c\<^sub>o\<^sub>n\<^sub>f"
+  proof -
+    have "\<lbrakk> \<Gamma>, n \<turnstile> (K\<^sub>1 time-delayed by \<delta>\<tau> on K\<^sub>2 implies K\<^sub>3) # \<Psi> \<triangleright> \<Phi> \<rbrakk>\<^sub>c\<^sub>o\<^sub>n\<^sub>f
+           = \<lbrakk>\<lbrakk> \<Gamma> \<rbrakk>\<rbrakk>\<^sub>s\<^sub>y\<^sub>m\<^sub>r\<^sub>u\<^sub>n \<inter> \<lbrakk>\<lbrakk> (K\<^sub>1 time-delayed by \<delta>\<tau> on K\<^sub>2 implies K\<^sub>3) # \<Psi> \<nabla> n \<rbrakk>\<rbrakk>\<^sub>T\<^sub>E\<^sub>S\<^sub>L \<inter> \<lbrakk>\<lbrakk> \<Phi> \<nabla> Suc n \<rbrakk>\<rbrakk>\<^sub>T\<^sub>E\<^sub>S\<^sub>L"
+      by simp
+    moreover have "\<lbrakk> K\<^sub>1 \<not>\<Up> n # \<Gamma>, n \<turnstile> \<Psi> \<triangleright> (K\<^sub>1 time-delayed by \<delta>\<tau> on K\<^sub>2 implies K\<^sub>3) # \<Phi> \<rbrakk>\<^sub>c\<^sub>o\<^sub>n\<^sub>f
+                     = \<lbrakk>\<lbrakk> K\<^sub>1 \<not>\<Up> n # \<Gamma> \<rbrakk>\<rbrakk>\<^sub>s\<^sub>y\<^sub>m\<^sub>r\<^sub>u\<^sub>n \<inter> \<lbrakk>\<lbrakk> \<Psi> \<nabla> n \<rbrakk>\<rbrakk>\<^sub>T\<^sub>E\<^sub>S\<^sub>L \<inter> \<lbrakk>\<lbrakk> (K\<^sub>1 time-delayed by \<delta>\<tau> on K\<^sub>2 implies K\<^sub>3) # \<Phi> \<nabla> Suc n \<rbrakk>\<rbrakk>\<^sub>T\<^sub>E\<^sub>S\<^sub>L"
+      by simp
+    moreover have "\<lbrakk> K\<^sub>1 \<Up> n # \<Gamma>, n \<turnstile> (K\<^sub>3 sporadic \<lfloor>\<tau>\<^sub>v\<^sub>a\<^sub>r(K\<^sub>2, n) \<oplus> \<delta>\<tau>\<rfloor> on K\<^sub>2) # \<Psi> \<triangleright> (K\<^sub>1 time-delayed by \<delta>\<tau> on K\<^sub>2 implies K\<^sub>3) # \<Phi> \<rbrakk>\<^sub>c\<^sub>o\<^sub>n\<^sub>f
+                     = \<lbrakk>\<lbrakk> K\<^sub>1 \<Up> n # \<Gamma> \<rbrakk>\<rbrakk>\<^sub>s\<^sub>y\<^sub>m\<^sub>r\<^sub>u\<^sub>n \<inter> \<lbrakk>\<lbrakk> (K\<^sub>3 sporadic \<lfloor>\<tau>\<^sub>v\<^sub>a\<^sub>r(K\<^sub>2, n) \<oplus> \<delta>\<tau>\<rfloor> on K\<^sub>2) # \<Psi> \<nabla> n \<rbrakk>\<rbrakk>\<^sub>T\<^sub>E\<^sub>S\<^sub>L
+                     \<inter> \<lbrakk>\<lbrakk> (K\<^sub>1 time-delayed by \<delta>\<tau> on K\<^sub>2 implies K\<^sub>3) # \<Phi> \<nabla> Suc n \<rbrakk>\<rbrakk>\<^sub>T\<^sub>E\<^sub>S\<^sub>L"
+      by simp
+    ultimately show ?thesis
+    proof -
+      have "\<lbrakk> \<Gamma>, n \<turnstile> (K\<^sub>1 time-delayed by \<delta>\<tau> on K\<^sub>2 implies K\<^sub>3) # \<Psi> \<triangleright> \<Phi> \<rbrakk>\<^sub>c\<^sub>o\<^sub>n\<^sub>f = \<lbrakk>\<lbrakk> \<Gamma> \<rbrakk>\<rbrakk>\<^sub>s\<^sub>y\<^sub>m\<^sub>r\<^sub>u\<^sub>n \<inter> (\<lbrakk>\<lbrakk> (K\<^sub>1 time-delayed by \<delta>\<tau> on K\<^sub>2 implies K\<^sub>3) # \<Psi> \<nabla> n \<rbrakk>\<rbrakk>\<^sub>T\<^sub>E\<^sub>S\<^sub>L \<inter> \<lbrakk>\<lbrakk> \<Phi> \<nabla> Suc n \<rbrakk>\<rbrakk>\<^sub>T\<^sub>E\<^sub>S\<^sub>L)"
+        using \<open>\<lbrakk> \<Gamma>, n \<turnstile> (K\<^sub>1 time-delayed by \<delta>\<tau> on K\<^sub>2 implies K\<^sub>3) # \<Psi> \<triangleright> \<Phi> \<rbrakk>\<^sub>c\<^sub>o\<^sub>n\<^sub>f = \<lbrakk>\<lbrakk> \<Gamma> \<rbrakk>\<rbrakk>\<^sub>s\<^sub>y\<^sub>m\<^sub>r\<^sub>u\<^sub>n \<inter> \<lbrakk>\<lbrakk> (K\<^sub>1 time-delayed by \<delta>\<tau> on K\<^sub>2 implies K\<^sub>3) # \<Psi> \<nabla> n \<rbrakk>\<rbrakk>\<^sub>T\<^sub>E\<^sub>S\<^sub>L \<inter> \<lbrakk>\<lbrakk> \<Phi> \<nabla> Suc n \<rbrakk>\<rbrakk>\<^sub>T\<^sub>E\<^sub>S\<^sub>L\<close> by blast
+      then have "\<lbrakk> \<Gamma>, n \<turnstile> (K\<^sub>1 time-delayed by \<delta>\<tau> on K\<^sub>2 implies K\<^sub>3) # \<Psi> \<triangleright> \<Phi> \<rbrakk>\<^sub>c\<^sub>o\<^sub>n\<^sub>f = (\<lbrakk> K\<^sub>1 \<not>\<Up> n \<rbrakk>\<^sub>s\<^sub>y\<^sub>m\<^sub>r\<^sub>u\<^sub>n \<union> \<lbrakk> K\<^sub>1 \<Up> n \<rbrakk>\<^sub>s\<^sub>y\<^sub>m\<^sub>r\<^sub>u\<^sub>n \<inter> \<lbrakk> K\<^sub>3 sporadic \<lfloor> \<tau>\<^sub>v\<^sub>a\<^sub>r (K\<^sub>2, n) \<oplus> \<delta>\<tau> \<rfloor> on K\<^sub>2 \<nabla> n \<rbrakk>\<^sub>T\<^sub>E\<^sub>S\<^sub>L) \<inter> (\<lbrakk>\<lbrakk> \<Gamma> \<rbrakk>\<rbrakk>\<^sub>s\<^sub>y\<^sub>m\<^sub>r\<^sub>u\<^sub>n \<inter> (\<lbrakk>\<lbrakk> \<Psi> \<nabla> n \<rbrakk>\<rbrakk>\<^sub>T\<^sub>E\<^sub>S\<^sub>L \<inter> \<lbrakk>\<lbrakk> (K\<^sub>1 time-delayed by \<delta>\<tau> on K\<^sub>2 implies K\<^sub>3) # \<Phi> \<nabla> Suc n \<rbrakk>\<rbrakk>\<^sub>T\<^sub>E\<^sub>S\<^sub>L))"
+        using TESL_interp_at_index_timedelayed_cases TESL_interpretation_at_index_cons_morph by blast
+      then show ?thesis
+        by auto
+    qed
+  qed
+
 
 find_theorems name: "operational_semantics_step"
 theorem completeness:
   shows "\<lbrakk> \<Gamma>, n \<turnstile> \<Psi> \<triangleright> \<Phi> \<rbrakk>\<^sub>c\<^sub>o\<^sub>n\<^sub>f = (\<Union>X\<in>\<F>\<^sub>n\<^sub>e\<^sub>x\<^sub>t (\<Gamma>, n \<turnstile> \<Psi> \<triangleright> \<Phi>). \<lbrakk> X \<rbrakk>\<^sub>c\<^sub>o\<^sub>n\<^sub>f)"
-(*
-  apply (rule Operational.operational_semantics_step.cases)
-  apply (auto)
-  proof -
-  show "([], Suc n, \<Psi>, \<Phi>) \<hookrightarrow> (\<tau>\<^sub>v\<^sub>a\<^sub>r (K\<^sub>1, n\<^sub>1) \<doteq> \<alpha> * \<tau> + \<beta> # \<gamma> # \<Gamma>, 0, \<Psi>, \<Phi>)"
-    sorry
+  proof (induct \<Psi>)
+    case Nil
+    then show ?case using Fnext_solve_instant by simp
+  next
+    case (Cons \<psi> \<Psi>)
+    then show ?case
+      proof (induct \<psi>)
+        case (Sporadic K \<tau>)
+        then show ?case
+          using HeronConf_interp_at_index_sporadic_cases Fnext_solve_sporadic by simp
+      next
+        case (SporadicOn K1 \<tau> K2)
+        then show ?case 
+          using HeronConf_interp_at_index_sporadicon_cases Fnext_solve_sporadicon by simp
+      next
+        case (TagRelation K1 \<alpha> K2 \<beta>)
+        then show ?case
+          using HeronConf_interp_at_index_tagrel_cases Fnext_solve_tagrel by simp
+      next
+        case (Implies K1 K2)
+        then show ?case
+          using HeronConf_interp_at_index_implies_cases Fnext_solve_implies by simp
+      next
+        case (TimeDelayedBy Kmast \<tau> Kmeas Kslave)
+        then show ?case
+          using HeronConf_interp_at_index_timedelayed_cases Fnext_solve_timedelayed by simp
+      qed
   qed
-*)
-  sorry
-  (* proof (rule operational_semantics_step.induct) *)
-
 
 (**) section \<open>Termination of instantaneous formulae elimination\<close> (**)
 (* Idea: A bounded monotonic sequence is convergent *)
@@ -244,16 +393,40 @@ primrec measure_interpretation :: "TESL_formula \<Rightarrow> nat" ("\<lbrakk>\<
                         _ sporadic _ on _ \<Rightarrow> 1 + \<lbrakk>\<lbrakk> \<Phi> \<rbrakk>\<rbrakk>\<^sub>m\<^sub>e\<^sub>a\<^sub>s
                       | _                 \<Rightarrow> 2 + \<lbrakk>\<lbrakk> \<Phi> \<rbrakk>\<rbrakk>\<^sub>m\<^sub>e\<^sub>a\<^sub>s)"
 
-lemma elimation_rules_strictly_decreasing:
-  assumes "\<Gamma>\<^sub>1, n \<turnstile> \<Psi>\<^sub>1 \<triangleright> \<Phi>\<^sub>1  \<hookrightarrow>  \<Gamma>\<^sub>2, n \<turnstile> \<Psi>\<^sub>2 \<triangleright> \<Phi>\<^sub>2"
-  shows "\<lbrakk>\<lbrakk> \<Psi>\<^sub>1 \<rbrakk>\<rbrakk>\<^sub>m\<^sub>e\<^sub>a\<^sub>s > \<lbrakk>\<lbrakk> \<Psi>\<^sub>2 \<rbrakk>\<rbrakk>\<^sub>m\<^sub>e\<^sub>a\<^sub>s"
-  by (insert assms, erule operational_semantics_step.cases, auto)
+fun measure_interpretation_config :: "config \<Rightarrow> nat" ("\<lbrakk>\<lbrakk> _ \<rbrakk>\<rbrakk>\<^sub>m\<^sub>e\<^sub>a\<^sub>s\<^sub>c\<^sub>o\<^sub>n\<^sub>f\<^sub>i\<^sub>g") where
+    "\<lbrakk>\<lbrakk> \<Gamma>, n \<turnstile> \<Psi> \<triangleright> \<Phi> \<rbrakk>\<rbrakk>\<^sub>m\<^sub>e\<^sub>a\<^sub>s\<^sub>c\<^sub>o\<^sub>n\<^sub>f\<^sub>i\<^sub>g = \<lbrakk>\<lbrakk> \<Psi> \<rbrakk>\<rbrakk>\<^sub>m\<^sub>e\<^sub>a\<^sub>s"
 
-theorem instant_computation_termination:
-  shows "wf \<hookrightarrow>\<^sub>e"
-  apply (rule wf_bounded_measure)
-(*apply (rule_tac ?ub="\<lambda>x. x" ?f="\<lambda>x. \<lbrakk>\<lbrakk> x \<rbrakk>\<rbrakk>\<^sub>m\<^sub>e\<^sub>a\<^sub>s" in wf_bounded_measure) *)
+lemma elimation_rules_strictly_decreasing:
+  assumes "\<Gamma>\<^sub>1, n\<^sub>1 \<turnstile> \<Psi>\<^sub>1 \<triangleright> \<Phi>\<^sub>1  \<hookrightarrow>\<^sub>e  \<Gamma>\<^sub>2, n\<^sub>2 \<turnstile> \<Psi>\<^sub>2 \<triangleright> \<Phi>\<^sub>2"
+  shows "\<lbrakk>\<lbrakk> \<Psi>\<^sub>1 \<rbrakk>\<rbrakk>\<^sub>m\<^sub>e\<^sub>a\<^sub>s > \<lbrakk>\<lbrakk> \<Psi>\<^sub>2 \<rbrakk>\<rbrakk>\<^sub>m\<^sub>e\<^sub>a\<^sub>s"
+  by (insert assms, erule operational_semantics_elim.cases, auto)
+
+lemma elimation_rules_strictly_decreasing_meas:
+  assumes "\<Gamma>\<^sub>1, n\<^sub>1 \<turnstile> \<Psi>\<^sub>1 \<triangleright> \<Phi>\<^sub>1  \<hookrightarrow>\<^sub>e  \<Gamma>\<^sub>2, n\<^sub>2 \<turnstile> \<Psi>\<^sub>2 \<triangleright> \<Phi>\<^sub>2"
+  shows "(\<Psi>\<^sub>2, \<Psi>\<^sub>1) \<in> measure measure_interpretation"
+  by (insert assms, erule operational_semantics_elim.cases, auto)
+
+lemma elimation_rules_strictly_decreasing_meas':
+  assumes "\<S>\<^sub>1  \<hookrightarrow>\<^sub>e  \<S>\<^sub>2"
+  shows "(\<S>\<^sub>2, \<S>\<^sub>1) \<in> measure measure_interpretation_config"
   sorry
+
+lemma instant_computation_termination:
+  shows "wf {(\<S>\<^sub>1, \<S>\<^sub>2). \<S>\<^sub>1 \<hookrightarrow>\<^sub>e \<S>\<^sub>2}"
+  apply (rule wf_subset)
+  proof -
+    have "measure (\<lambda>\<S>. \<lbrakk>\<lbrakk> \<S> \<rbrakk>\<rbrakk>\<^sub>m\<^sub>e\<^sub>a\<^sub>s\<^sub>c\<^sub>o\<^sub>n\<^sub>f\<^sub>i\<^sub>g) = { (\<S>\<^sub>1, \<S>\<^sub>2). \<lbrakk>\<lbrakk> \<S>\<^sub>1 \<rbrakk>\<rbrakk>\<^sub>m\<^sub>e\<^sub>a\<^sub>s\<^sub>c\<^sub>o\<^sub>n\<^sub>f\<^sub>i\<^sub>g < \<lbrakk>\<lbrakk> \<S>\<^sub>2 \<rbrakk>\<rbrakk>\<^sub>m\<^sub>e\<^sub>a\<^sub>s\<^sub>c\<^sub>o\<^sub>n\<^sub>f\<^sub>i\<^sub>g }"
+      by (simp add: inv_image_def less_eq measure_def)
+    show "{(\<S>\<^sub>1, \<S>\<^sub>2). \<S>\<^sub>1 \<hookrightarrow>\<^sub>e \<S>\<^sub>2} \<subseteq> (measure (\<lambda>\<S>. \<lbrakk>\<lbrakk> \<S> \<rbrakk>\<rbrakk>\<^sub>m\<^sub>e\<^sub>a\<^sub>s\<^sub>c\<^sub>o\<^sub>n\<^sub>f\<^sub>i\<^sub>g))"
+      sorry  (* Pas dans le bon sens !?! *)
+    show "wf (measure measure_interpretation_config)"
+      by simp
+  qed
+
+theorem instant_computation_termination':
+  shows "wfP (\<lambda>\<S>\<^sub>1 \<S>\<^sub>2. \<S>\<^sub>1 \<hookrightarrow>\<^sub>e \<S>\<^sub>2)"
+  using instant_computation_termination
+  by (simp add: wfP_def)
 
 lemma run_index_progress:
   assumes "\<Gamma>\<^sub>1, n\<^sub>1 \<turnstile> \<Psi>\<^sub>1 \<triangleright> \<Phi>\<^sub>1  \<hookrightarrow>  \<Gamma>\<^sub>2, n\<^sub>2 \<turnstile> \<Psi>\<^sub>2 \<triangleright> \<Phi>\<^sub>2"
@@ -261,14 +434,10 @@ lemma run_index_progress:
   by (insert assms, erule operational_semantics_step.cases, auto)
 
 lemma run_index_progress_simlstep:
-  assumes "(\<Gamma>\<^sub>1, n\<^sub>1 \<turnstile> \<Psi>\<^sub>1 \<triangleright> \<Phi>\<^sub>1, \<Gamma>\<^sub>2, n\<^sub>2 \<turnstile> \<Psi>\<^sub>2 \<triangleright> \<Phi>\<^sub>2) \<in> \<hookrightarrow>\<^sub>\<nabla>"
+  assumes "\<Gamma>\<^sub>1, n\<^sub>1 \<turnstile> \<Psi>\<^sub>1 \<triangleright> \<Phi>\<^sub>1  \<hookrightarrow>\<^sub>\<nabla>  \<Gamma>\<^sub>2, n\<^sub>2 \<turnstile> \<Psi>\<^sub>2 \<triangleright> \<Phi>\<^sub>2"
   shows "n\<^sub>2 = Suc n\<^sub>1"
   apply (insert assms)
-  apply auto
   sorry
-
-(**) section \<open>Semidecidability\<close> (**)
-
 
 (**) section \<open>Composition\<close> (**)
 
@@ -277,13 +446,8 @@ lemma composition:
          = \<lbrakk> \<Gamma>\<^sub>1 @ \<Gamma>\<^sub>2, n \<turnstile> \<Psi>\<^sub>1 @ \<Psi>\<^sub>2 \<triangleright> \<Phi>\<^sub>1 @ \<Phi>\<^sub>2 \<rbrakk>\<^sub>c\<^sub>o\<^sub>n\<^sub>f"
   using TESL_interp_at_index_composition symrun_interp_expansion by auto
 
-lemma sat_composition:
-  assumes "K\<^sub>1 time-delayed by \<delta>\<tau> on K\<^sub>2 implies K\<^sub>3 \<notin> set \<Phi> \<union> set \<Phi>'"
-  assumes "\<TTurnstile> \<Gamma>\<^sub>1, n \<turnstile> [] \<triangleright> \<Phi>\<^sub>1"
-  assumes "\<TTurnstile> \<Gamma>\<^sub>2, n \<turnstile> [] \<triangleright> \<Phi>\<^sub>2"
-  assumes "consistency_run (\<Gamma>\<^sub>1 @ \<Gamma>\<^sub>2)"
-  shows   "\<TTurnstile> \<Gamma>\<^sub>1 @ \<Gamma>\<^sub>2, n \<turnstile> [] \<triangleright> \<Phi>\<^sub>1 @ \<Phi>\<^sub>2"
-  oops
+(**) section \<open>Semidecidability\<close> (**)
+(* The set of runs hence becomes recursively countable due to the previous observations. *)
 
 (**) section \<open>Existence\<close> (**)
 fun tagrel_consistent :: "TESL_formula \<Rightarrow> bool" where
