Operational.thy
@@ -7,11 +7,10 @@ begin
 text{* Operational steps *}
 
 abbreviation uncurry_conf
-  :: "system \<Rightarrow> instant_index \<Rightarrow> TESL_formula \<Rightarrow> TESL_formula \<Rightarrow> config" ("_, _ \<turnstile> _ \<triangleright> _" 50) where
+  :: "system \<Rightarrow> instant_index \<Rightarrow> TESL_formula \<Rightarrow> TESL_formula \<Rightarrow> config" ("_, _ \<turnstile> _ \<triangleright> _" 80) where
   "\<Gamma>, n \<turnstile> \<Psi> \<triangleright> \<Phi> \<equiv> (\<Gamma>, n, \<Psi>, \<Phi>)"
 
-inductive operational_semantics_step
-  :: "config \<Rightarrow> config \<Rightarrow> bool" ("_ \<hookrightarrow> _" 50) where
+inductive operational_semantics_step :: "config \<Rightarrow> config \<Rightarrow> bool" ("_ \<hookrightarrow> _" 70) where
   instant_i:
   "consistent_run \<Gamma> \<Longrightarrow>
    \<Gamma>, n \<turnstile> [] \<triangleright> \<Phi>
@@ -53,49 +52,83 @@ inductive operational_semantics_step
    \<Gamma>, n \<turnstile> (K\<^sub>1 time-delayed by \<delta>\<tau> on K\<^sub>2 implies K\<^sub>3) # \<Psi> \<triangleright> \<Phi>
      \<hookrightarrow>  K\<^sub>1 \<Up> n # \<Gamma>, n \<turnstile> (K\<^sub>3 sporadic \<lfloor>\<tau>\<^sub>v\<^sub>a\<^sub>r(K\<^sub>2, n) \<oplus> \<delta>\<tau>\<rfloor> on K\<^sub>2) # \<Psi> \<triangleright> (K\<^sub>1 time-delayed by \<delta>\<tau> on K\<^sub>2 implies K\<^sub>3) # \<Phi>"
 
-abbreviation operational_semantics_rellifted
-  :: "config rel" ("\<hookrightarrow>\<^sup>\<up>") where
-  "\<hookrightarrow>\<^sup>\<up> \<equiv> { ((\<Gamma>\<^sub>1, n\<^sub>1, \<Psi>\<^sub>1, \<Phi>\<^sub>1), (\<Gamma>\<^sub>2, n\<^sub>2, \<Psi>\<^sub>2, \<Phi>\<^sub>2)).
-              \<Gamma>\<^sub>1, n\<^sub>1 \<turnstile> \<Psi>\<^sub>1 \<triangleright> \<Phi>\<^sub>1 \<hookrightarrow> \<Gamma>\<^sub>2, n\<^sub>2 \<turnstile> \<Psi>\<^sub>2 \<triangleright> \<Phi>\<^sub>2 }"
+inductive operational_semantics_intro :: "config \<Rightarrow> config \<Rightarrow> bool" ("_ \<hookrightarrow>\<^sub>i _" 70) where
+  instant_i:
+  "consistent_run \<Gamma> \<Longrightarrow>
+   \<Gamma>, n \<turnstile> [] \<triangleright> \<Phi>
+     \<hookrightarrow>\<^sub>i  \<Gamma>, Suc n \<turnstile> \<Phi> \<triangleright> []"
 
-lemma rel_uncurry_equiv:
-  shows "(\<S>\<^sub>1, \<S>\<^sub>2) \<in> \<hookrightarrow>\<^sup>\<up> \<longleftrightarrow> \<S>\<^sub>1 \<hookrightarrow> \<S>\<^sub>2"
-  by auto
+inductive operational_semantics_elim :: "config \<Rightarrow> config \<Rightarrow> bool" ("_ \<hookrightarrow>\<^sub>e _" 70) where
+  sporadic_e1:
+  "consistent_run \<Gamma> \<Longrightarrow>
+   \<Gamma>, n \<turnstile> (K sporadic \<tau>) # \<Psi> \<triangleright> \<Phi>
+     \<hookrightarrow>\<^sub>e  \<Gamma>, n \<turnstile> \<Psi> \<triangleright> (K sporadic \<tau>) # \<Phi>"
+| sporadic_e2:
+  "consistent_run ((K \<Up> n) # (K \<Down> n @ \<lfloor>\<tau>\<rfloor>) # \<Gamma>) \<Longrightarrow>
+   \<Gamma>, n \<turnstile> (K sporadic \<tau>) # \<Psi> \<triangleright> \<Phi>
+     \<hookrightarrow>\<^sub>e  K \<Up> n # K \<Down> n @ \<lfloor>\<tau>\<rfloor> # \<Gamma>, n \<turnstile> \<Psi> \<triangleright> \<Phi>"
+| sporadic_on_e1:
+  "consistent_run \<Gamma> \<Longrightarrow>
+   \<Gamma>, n \<turnstile> (K\<^sub>1 sporadic \<tau> on K\<^sub>2) # \<Psi> \<triangleright> \<Phi>
+     \<hookrightarrow>\<^sub>e  \<Gamma>, n \<turnstile> \<Psi> \<triangleright> (K\<^sub>1 sporadic \<tau> on K\<^sub>2) # \<Phi>"
+| sporadic_on_e2:
+  "consistent_run ((K\<^sub>1 \<Up> n) # (K\<^sub>2 \<Down> n @ \<tau>) # \<Gamma>) \<Longrightarrow>
+   \<Gamma>, n \<turnstile> (K\<^sub>1 sporadic \<tau> on K\<^sub>2) # \<Psi> \<triangleright> \<Phi>
+     \<hookrightarrow>\<^sub>e  K\<^sub>1 \<Up> n # K\<^sub>2 \<Down> n @ \<tau> # \<Gamma>, n \<turnstile> \<Psi> \<triangleright> \<Phi>"
+| tagrel_e:
+  "consistent_run ((\<tau>\<^sub>v\<^sub>a\<^sub>r(K\<^sub>1, n) \<doteq> \<alpha> * \<tau>\<^sub>v\<^sub>a\<^sub>r(K\<^sub>2, n) + \<beta>) # \<Gamma>) \<Longrightarrow>
+   \<Gamma>, n \<turnstile> (tag-relation K\<^sub>1 = \<alpha> * K\<^sub>2 + \<beta>) # \<Psi> \<triangleright> \<Phi>
+     \<hookrightarrow>\<^sub>e  (\<tau>\<^sub>v\<^sub>a\<^sub>r(K\<^sub>1, n) \<doteq> \<alpha> * \<tau>\<^sub>v\<^sub>a\<^sub>r(K\<^sub>2, n) + \<beta>) # \<Gamma>, n \<turnstile> \<Psi> \<triangleright> (tag-relation K\<^sub>1 = \<alpha> * K\<^sub>2 + \<beta>) # \<Phi>"
+| implies_e1:
+  "consistent_run (K\<^sub>1 \<not>\<Up> n # \<Gamma>) \<Longrightarrow>
+   \<Gamma>, n \<turnstile> (K\<^sub>1 implies K\<^sub>2) # \<Psi> \<triangleright> \<Phi>
+     \<hookrightarrow>\<^sub>e  K\<^sub>1 \<not>\<Up> n # \<Gamma>, n \<turnstile> \<Psi> \<triangleright> (K\<^sub>1 implies K\<^sub>2) # \<Phi>"
+| implies_e2:
+  "consistent_run ((K\<^sub>1 \<Up> n) # (K\<^sub>2 \<Up> n) # \<Gamma>) \<Longrightarrow>
+   \<Gamma>, n \<turnstile> (K\<^sub>1 implies K\<^sub>2) # \<Psi> \<triangleright> \<Phi>
+     \<hookrightarrow>\<^sub>e  K\<^sub>1 \<Up> n # K\<^sub>2 \<Up> n # \<Gamma>, n \<turnstile> \<Psi> \<triangleright> (K\<^sub>1 implies K\<^sub>2) # \<Phi>"
+| timedelayed_e1:
+  "consistent_run (K\<^sub>1 \<not>\<Up> n # \<Gamma>) \<Longrightarrow>
+   \<Gamma>, n \<turnstile> (K\<^sub>1 time-delayed by \<delta>\<tau> on K\<^sub>2 implies K\<^sub>3) # \<Psi> \<triangleright> \<Phi>
+     \<hookrightarrow>\<^sub>e  K\<^sub>1 \<not>\<Up> n # \<Gamma>, n \<turnstile> \<Psi> \<triangleright> (K\<^sub>1 time-delayed by \<delta>\<tau> on K\<^sub>2 implies K\<^sub>3) # \<Phi>"
+| timedelayed_e2:
+  "consistent_run (K\<^sub>1 \<Up> n # \<Gamma>) \<Longrightarrow>
+   \<Gamma>, n \<turnstile> (K\<^sub>1 time-delayed by \<delta>\<tau> on K\<^sub>2 implies K\<^sub>3) # \<Psi> \<triangleright> \<Phi>
+     \<hookrightarrow>\<^sub>e  K\<^sub>1 \<Up> n # \<Gamma>, n \<turnstile> (K\<^sub>3 sporadic \<lfloor>\<tau>\<^sub>v\<^sub>a\<^sub>r(K\<^sub>2, n) \<oplus> \<delta>\<tau>\<rfloor> on K\<^sub>2) # \<Psi> \<triangleright> (K\<^sub>1 time-delayed by \<delta>\<tau> on K\<^sub>2 implies K\<^sub>3) # \<Phi>"
 
-abbreviation operational_semantics_rellifted_elim
-  :: "config rel" ("\<hookrightarrow>\<^sub>e") where
-  "\<hookrightarrow>\<^sub>e \<equiv> { ((\<Gamma>\<^sub>1, n, \<Psi>\<^sub>1, \<Phi>\<^sub>1), (\<Gamma>\<^sub>2, n, \<Psi>\<^sub>2, \<Phi>\<^sub>2)).
-              \<Gamma>\<^sub>1, n \<turnstile> \<Psi>\<^sub>1 \<triangleright> \<Phi>\<^sub>1 \<hookrightarrow> \<Gamma>\<^sub>2, n \<turnstile> \<Psi>\<^sub>2 \<triangleright> \<Phi>\<^sub>2 }"
+find_theorems name:"operational_semantics_step"
 
-abbreviation operational_semantics_rellifted_intro
-  :: "config rel" ("\<hookrightarrow>\<^sub>i") where
-  "\<hookrightarrow>\<^sub>i \<equiv> { ((\<Gamma>\<^sub>1, n\<^sub>1, \<Psi>\<^sub>1, \<Phi>\<^sub>1), (\<Gamma>\<^sub>2, n\<^sub>2, \<Psi>\<^sub>2, \<Phi>\<^sub>2)).
-              n\<^sub>2 = Suc n\<^sub>1
-              \<and> \<Gamma>\<^sub>1, n\<^sub>1 \<turnstile> \<Psi>\<^sub>1 \<triangleright> \<Phi>\<^sub>1 \<hookrightarrow> \<Gamma>\<^sub>2, n\<^sub>2 \<turnstile> \<Psi>\<^sub>2 \<triangleright> \<Phi>\<^sub>2 }"
+lemma operational_semantics_split:
+  shows "\<S>\<^sub>1 \<hookrightarrow> \<S>\<^sub>2 = \<S>\<^sub>1 \<hookrightarrow>\<^sub>i \<S>\<^sub>2 \<or> \<S>\<^sub>1 \<hookrightarrow>\<^sub>e \<S>\<^sub>2"
+  apply (rule operational_semantics_step.induct)
+  defer
+  apply (simp add: operational_semantics_intro.instant_i operational_semantics_step.instant_i)
+  apply (simp add: operational_semantics_elim.sporadic_e1)
+  apply (simp add: operational_semantics_elim.sporadic_e2)
+  apply (simp add: operational_semantics_elim.sporadic_on_e1)
+  apply (simp add: operational_semantics_elim.sporadic_on_e2)
+  apply (simp add: operational_semantics_elim.tagrel_e)
+  apply (simp add: operational_semantics_elim.implies_e1)
+  apply (simp add: operational_semantics_elim.implies_e2)
+  apply (simp add: operational_semantics_elim.timedelayed_e1)
+  apply (simp add: operational_semantics_elim.timedelayed_e2)
+  sorry
 
-abbreviation operational_semantics_simulation_step
-  :: "config rel" ("\<hookrightarrow>\<^sub>\<nabla>") where
-  "\<hookrightarrow>\<^sub>\<nabla> \<equiv> { ((\<Gamma>\<^sub>1, n\<^sub>1, \<Psi>, \<Phi>\<^sub>1), (\<Gamma>\<^sub>2, n\<^sub>2, \<Psi>, \<Phi>\<^sub>2)).
-                \<Psi> = []
-              \<and> (\<Gamma>\<^sub>1, n\<^sub>1 \<turnstile> \<Psi> \<triangleright> \<Phi>\<^sub>1, \<Gamma>\<^sub>2, n\<^sub>2 \<turnstile> \<Psi> \<triangleright> \<Phi>\<^sub>2) \<in> \<hookrightarrow>\<^sup>\<up>\<^sup>+
-              \<and> consistent_run \<Gamma>\<^sub>1
-              \<and> consistent_run \<Gamma>\<^sub>2}"
+abbreviation operational_semantics_step_rtranclp :: "config \<Rightarrow> config \<Rightarrow> bool" ("_ \<hookrightarrow>\<^sup>*\<^sup>* _" 70) where
+  "A \<hookrightarrow>\<^sup>*\<^sup>* B \<equiv> operational_semantics_step\<^sup>*\<^sup>* A B"
 
-(* Example of one simulation step: introduction rule then one elimination *)
-(* Note that \<hookrightarrow>\<^sub>\<nabla> is unfolded as necessary as it is to eliminate \<psi>-formulae *)
-lemma "([], 0        \<turnstile> [] \<triangleright> [H\<^sub>1 sporadic \<tau>\<^sub>i\<^sub>n\<^sub>t 0, H\<^sub>1 implies H\<^sub>2],
-         \<Gamma>, 1 \<turnstile> [] \<triangleright> \<Phi>)
-         \<in> \<hookrightarrow>\<^sub>\<nabla>"
-apply auto
-apply (rule trancl_into_trancl)
-apply (rule trancl_into_trancl)
-apply (rule r_into_trancl)
-apply simp
-apply (rule instant_i)
-  apply (rule witness_consistency, auto, ((simp add: Abs_run_inverse_rewrite mono_iff_le_Suc)+)?)
-apply (rule sporadic_e2)
-  apply (rule witness_consistency, auto, ((simp add: Abs_run_inverse_rewrite mono_iff_le_Suc)+)?)
-sorry (* OK *)
+abbreviation operational_semantics_step_tranclp :: "config \<Rightarrow> config \<Rightarrow> bool" ("_ \<hookrightarrow>\<^sup>+\<^sup>+ _" 70) where
+  "A \<hookrightarrow>\<^sup>+\<^sup>+ B \<equiv> operational_semantics_step\<^sup>+\<^sup>+ A B"
+
+abbreviation operational_semantics_step_reflclp :: "config \<Rightarrow> config \<Rightarrow> bool" ("_ \<hookrightarrow>\<^sup>=\<^sup>= _" 70) where
+  "A \<hookrightarrow>\<^sup>=\<^sup>= B \<equiv> operational_semantics_step\<^sup>=\<^sup>= A B"
+
+abbreviation operational_semantics_step_relpowp :: "config \<Rightarrow> nat \<Rightarrow> config \<Rightarrow> bool" ("_ \<hookrightarrow>\<^bsup>_\<^esup> _" 70) where
+  "A \<hookrightarrow>\<^bsup>n\<^esup> B \<equiv> (operational_semantics_step ^^ n) A B"
+
+inductive operational_semantics_simlstep :: "config \<Rightarrow> config \<Rightarrow> bool" ("_ \<hookrightarrow>\<^sub>\<nabla> _" 70) where
+  "(\<Gamma>\<^sub>1, n \<turnstile> [] \<triangleright> \<Phi>\<^sub>1) \<hookrightarrow>\<^sup>+\<^sup>+ (\<Gamma>, n + 1 \<turnstile> [] \<triangleright> \<Phi>\<^sub>2) \<Longrightarrow>
+   (\<Gamma>\<^sub>1, n \<turnstile> [] \<triangleright> \<Phi>\<^sub>1) \<hookrightarrow>\<^sub>\<nabla> (\<Gamma>, n + 1 \<turnstile> [] \<triangleright> \<Phi>\<^sub>2)"
 
 inductive finite_SAT :: "config \<Rightarrow> bool" ("\<TTurnstile> _" 50) where
   finite_SAT_ax: "set (NoSporadic \<Phi>) = set \<Phi> \<Longrightarrow>
